define count for 2.3, need to discuss importing libraries

ConcreteSemanticsLean/ch2.lean
@@ -1,10 +1,31 @@
 import ConcreteSemanticsLean.cslib
+import Init.Prelude
 
 -- 2.1
 
 -- 2.2
 
 -- 2.3
+def count [DecidableEq X] (elm : X) (l : mylist X) (occ : Nat) : Nat :=
+  match l with
+  | [] => occ
+  | a :: l' => if elm = a then count elm l' (occ + 1) else count elm l' occ
+
+#eval count 1 (1 :: 2 :: 1 :: []) 0 -- 2
+#eval count 3 (1 :: 2 :: 1 :: []) 0 -- 0
+#eval count type1.A type1_list 0 -- 1
+
+-- someone should try to find  way to remove the need for DecidableEq
+theorem count_x_le_len [DecidableEq X] : ∀ (elm : X) (l : mylist X), count elm l 0 ≤ len l := by
+  intros elm l
+  induction l
+  . simp [count, len]
+  . simp [count, len]
+    sorry
+
+
+
+
 
 -- 2.4
 
